fstar/new/NetworkBinder.fst
@@ -9,3 +9,9 @@ let network_to_option #a opt =
   | None_nt -> return None
   | Some_nt x -> return (Some x)
   | _ -> fail "network_to_option: not a valid option"
+
+val option_to_network: #a:Type -> option a -> option_nt a
+let option_to_network #a opt =
+  match opt with
+  | None -> None_nt
+  | Some x -> Some_nt x
