fstar/new/TreeDEM.Message.Transcript.fst
@@ -1,0 +1,43 @@
+module TreeDEM.Message.Transcript
+
+open TreeDEM.Message.Framing
+open TreeDEM.Message.Content
+open NetworkTypes
+open Lib.ByteSequence
+open Lib.IntTypes
+open Parser
+open Lib.Result
+open Crypto
+
+val compute_confirmed_transcript_hash: cs:ciphersuite -> message -> bytes -> bytes -> result (lbytes (hash_length cs))
+let compute_confirmed_transcript_hash cs msg signature interim_transcript_hash =
+  if not (Seq.length msg.m_group_id < 256) then
+    fail "compute_confirmed_transcript_hash: group_id too long"
+  else if not (msg.m_epoch < pow2 64) then
+    fail "compute_confirmed_transcript_hash: epoch too big"
+  else if not (Seq.length msg.m_authenticated_data < pow2 32) then
+    fail "compute_confirmed_transcript_hash: authenticated_data too long"
+  else if not (Seq.length signature < pow2 16) then
+    fail "compute_confirmed_transcript_hash: signature too long"
+  else (
+    sender <-- sender_to_network msg.m_sender;
+    content <-- message_content_to_network cs msg.m_message_content;
+    let serialized_msg = ps_mls_plaintext_commit_content.serialize ({
+      mpccn_group_id = msg.m_group_id;
+      mpccn_epoch = u64 msg.m_epoch;
+      mpccn_sender = sender;
+      mpccn_authenticated_data = msg.m_authenticated_data;
+      mpccn_content = content;
+      mpccn_signature = signature;
+    }) in
+    hash_hash cs (Seq.append interim_transcript_hash serialized_msg)
+  )
+
+val compute_interim_transcript_hash: cs:ciphersuite -> message_auth -> bytes -> result (lbytes (hash_length cs))
+let compute_interim_transcript_hash cs msg_auth confirmed_transcript_hash =
+  confirmation_tag <-- opt_bytes_to_opt_tag msg_auth.m_confirmation_tag;
+  let serialized_auth = ps_mls_plaintext_commit_auth_data.serialize ({
+    mpcadn_confirmation_tag = confirmation_tag;
+  }) in
+  hash_hash cs (Seq.append confirmed_transcript_hash serialized_auth)
+
